sum random

sum-random/manual/SumRandom_Update.thy
@@ -6,24 +6,54 @@ begin
 context SumRandom begin
 
 section random_with_seed
+(*
 
-                                                 
+
+definition
+  abbreviatedType1 :: " Cogent.type"
+where
+  "abbreviatedType1 \<equiv> 
+      TRecord [(''seed'',  (TPrim (Num U64), Present)), 
+               (''value'', (TPrim (Num U64), Present))] Unboxed"
+
+lemmas abbreviated_type_defs =
+  abbreviatedType1_def
+
+definition
+  rand_with_seed_type :: " Cogent.kind list \<times>  Cogent.type \<times>  Cogent.type"
+where
+  "rand_with_seed_type \<equiv> ([], (TPrim (Num U64), abbreviatedType1))"
+
+*)
+thm rand_with_seed'_def
+term rand_with_seed'        
+term val_rel
+term "rand_with_seed' 1"
+find_theorems val_rel
+
+print_locale SumRandom
+print_locale Random_seed_cogent_shallow
+
+thm Random_seed_ACInstall.random_seed.rand_with_seed'_ac_corres
+find_theorems "_::((lifted_globals, 'a) nondet_monad \<Rightarrow>_)"
 definition rand_with_seed_u:: "(funtyp, abstyp, ptrtyp) ufundef" where
   "rand_with_seed_u x y \<equiv>
       let (\<sigma>, s) = x;
          (\<sigma>', sv) = y
-      in \<exists>  (p::ptrtyp)  (v::8 word) (seed::ptrtyp) (seed'::ptrtyp). 
-           s = UPtr p (RCon ''Seed'' []) \<and>
-           sv =  URecord [ (UPtr p (RCon ''Seed'' []), RPtr (RCon ''Seed'' [])),
-                           (UPrim (LU8 v), RPrim (Num U8))] \<and> 
-           \<sigma> p = Some (UAbstract (Abs_utyp (TSeed seed)))\<and>
-           \<sigma>' = \<sigma>(p := Some (UAbstract (Abs_utyp (TSeed seed'))))"
+     
+      in 
+         \<exists> (seed::8 word) (seed'::8 word) (v::8 word) . 
+           s = UPrim (LU8 seed) \<and>
+           sv = URecord [ (UPrim (LU8 seed'), RPrim (Num U8)), 
+                           (UPrim (LU8 v), RPrim (Num U8))] \<and>
+           val_rel 
+           \<sigma>' = \<sigma>"
 
 lemma rand_with_seed_u_preservation:
   "\<lbrakk>upd.uval_typing \<Xi>' \<sigma> v (TCon ''WordArray'' [t] (Boxed ReadOnly ptrl)) r w;
     rand_with_seed_u (\<sigma>, v) (\<sigma>', v')\<rbrakk>
     \<Longrightarrow> \<exists>r' w'. upd.uval_typing \<Xi>' \<sigma>' v' (TPrim (Num U32)) r' w' \<and> r' \<subseteq> r \<and> upd.frame \<sigma> w \<sigma>' w'"
-  by (fastforce simp: rand_with_seed_u_def elim: upd.uval_typing.cases)
+  apply ( simp add: rand_with_seed_u_def elim: upd.uval_typing.cases)
 
 end (* of context *)
 
